update OpalSemantics with newer opal semantics -- incomplete

src/OpalSemantics.v
@@ -1,286 +1,477 @@
-Require Import String ListSet CpdtTactics.
+Require Import String ListSet CpdtTactics ListSet Wf FMapList
+        Coq.Structures.OrderedTypeEx String.
+
+Axiom proof_irrelevance :
+  forall (P : Prop) (p q : P), p = q.
 
 Definition var := string.
+Definition node := string.
 Definition world := string.
+Definition op := string.
 
 Inductive sexp :=
 | EmptySet : sexp
-| Var      : var -> sexp
-| Cons     : sexp -> sexp -> sexp
-| Extend   : sexp -> sexp -> sexp.
+| Var      : node -> var -> sexp
+| Cons     : sexp -> sexp -> sexp.
 
 Inductive sexp_is_value : sexp -> Prop :=
 | EmptySetIsValue : sexp_is_value EmptySet
 | ConsValuesIsValue : forall s1 s2,
     sexp_is_value s1 -> sexp_is_value s2 -> sexp_is_value (Cons s1 s2).
+Hint Constructors sexp_is_value.
 
-Definition sexp_value := {s: sexp | sexp_is_value s}.
-
-Inductive sexp_evaluation_context :=
-| SexpHole : sexp_evaluation_context
-| ConsLeft : sexp_evaluation_context -> sexp -> sexp_evaluation_context
-| ConsRight : sexp_value -> sexp_evaluation_context -> sexp_evaluation_context
-| ExtendLeft : sexp_evaluation_context -> sexp -> sexp_evaluation_context
-| ExtendRight : sexp_value -> sexp_evaluation_context -> sexp_evaluation_context.
-
-Fixpoint sexp_of_context (ctx: sexp_evaluation_context) (s: sexp) :=
-  match ctx with
-  | SexpHole => s
-  | ConsLeft ctx' r => Cons (sexp_of_context ctx' s) r
-  | ConsRight l ctx' => Cons (proj1_sig l) (sexp_of_context ctx' s)
-  | ExtendLeft ctx' r => Extend (sexp_of_context ctx' s) r
-  | ExtendRight l ctx' => Extend (proj1_sig l) (sexp_of_context ctx' s)
-  end.
+Definition sexp_value := {sexp | sexp_is_value sexp}.
 
 Inductive bool :=
-| Eq : sexp -> sexp -> bool
-| Mem : sexp -> sexp -> bool
-| Conj : bool -> bool -> bool
-| Disj : bool -> bool -> bool
-| True : bool
+| Eq    : sexp -> sexp -> bool
+| Mem   : sexp -> sexp -> bool
+| Conj  : bool -> bool -> bool
+| Disj  : bool -> bool -> bool
+| True  : bool
 | False : bool.
 
-Definition bool_value := {b: bool | b = True \/ b = False}.
+Inductive bool_is_psuedovalue : bool -> Prop :=
+| TruePsuedoValue : bool_is_psuedovalue True
+| FalsePsuedoValue : bool_is_psuedovalue False
+| MemPsuedoValue : forall l r, sexp_is_value l -> sexp_is_value r ->
+                               bool_is_psuedovalue (Mem l r)
+| EqPsuedoValue : forall l r, sexp_is_value l -> sexp_is_value r ->
+                              bool_is_psuedovalue (Eq l r)
+| ConjPsuedoValue : forall l r, bool_is_psuedovalue l -> bool_is_psuedovalue r ->
+                                bool_is_psuedovalue (Conj l r)
+| DisjPsuedoValue : forall l r, bool_is_psuedovalue l -> bool_is_psuedovalue r ->
+                                bool_is_psuedovalue (Disj l r).
+Hint Constructors bool_is_psuedovalue.
 
-Inductive bool_sexp_evaluation_context :=
-| BoolSexpMemLeft : sexp -> bool_sexp_evaluation_context
-| BoolSexpMemRight : sexp_value -> bool_sexp_evaluation_context
-| BoolSexpEqLeft : sexp -> bool_sexp_evaluation_context
-| BoolSexpEqRight : sexp_value -> bool_sexp_evaluation_context
-| BoolSexpConjLeft : bool_sexp_evaluation_context -> bool -> bool_sexp_evaluation_context
-| BoolSexpConjRight : bool_value -> bool_sexp_evaluation_context -> bool_sexp_evaluation_context
-| BoolSexpDisjLeft : bool_sexp_evaluation_context -> bool -> bool_sexp_evaluation_context
-| BoolSexpDisjRight : bool_value -> bool_sexp_evaluation_context -> bool_sexp_evaluation_context.
-
-Fixpoint bool_of_bool_sexp_context (ctx: bool_sexp_evaluation_context) (s: sexp) :=
-  match ctx with
-  | BoolSexpMemLeft r => Mem s r
-  | BoolSexpMemRight lvp => Mem (proj1_sig lvp) s
-  | BoolSexpEqLeft r => Eq s r
-  | BoolSexpEqRight lvp => Eq (proj1_sig lvp) s
-  | BoolSexpConjLeft ctx' r => Conj (bool_of_bool_sexp_context ctx' s) r
-  | BoolSexpConjRight lvp ctx' => Conj (proj1_sig lvp) (bool_of_bool_sexp_context ctx' s)
-  | BoolSexpDisjLeft ctx' r => Disj (bool_of_bool_sexp_context ctx' s) r
-  | BoolSexpDisjRight lvp ctx' => Disj (proj1_sig lvp) (bool_of_bool_sexp_context ctx' s)
-  end.
-
-Inductive bool_evaluation_context :=
-| BoolHole : bool_evaluation_context
-| ConjLeft : bool_evaluation_context -> bool -> bool_evaluation_context
-| ConjRight : bool_value -> bool_evaluation_context -> bool_evaluation_context
-| DisjLeft : bool_evaluation_context -> bool -> bool_evaluation_context
-| DisjRight : bool_value -> bool_evaluation_context -> bool_evaluation_context.
-
-Fixpoint bool_of_bool_context (ctx: bool_evaluation_context) (b: bool) :=
-  match ctx with
-  | BoolHole => b
-  | ConjLeft ctx' r => Conj (bool_of_bool_context ctx' b) r
-  | ConjRight lvp ctx' => Conj (proj1_sig lvp) (bool_of_bool_context ctx' b)
-  | DisjLeft ctx' r => Disj (bool_of_bool_context ctx' b) r
-  | DisjRight lvp ctx' => Disj (proj1_sig lvp) (bool_of_bool_context ctx' b)
-  end.
+Definition bool_psuedovalue := { b: bool | bool_is_psuedovalue b}.
+Definition bool_value := { b: bool | b = True \/ b = False}.
 
 Inductive com :=
-| Skip : com
-| If : bool -> com -> com -> com
-| Assign : var -> sexp -> com
-| Seq : com -> com -> com
-| Print : sexp -> com
-| Hyp : world -> com -> com
-| Commit : world -> com.
+| Skip   : com
+| Seq    : com -> com -> com
+| If     : bool -> com -> com -> com
+| With   : node -> com -> com
+| At   : node -> com -> com
+| Hyp    : world -> com -> com
+| Commit : world -> com
+| Handle : node -> var -> op -> sexp -> sexp -> com -> com
+| Op     : op -> com.
 
-Definition env := var -> nat -> sexp_value.
-Definition empty_env : env := (fun var idx => (exist _ EmptySet EmptySetIsValue)).
-Definition set_env (e: env) (v: var) (i: nat) (s: sexp_value) : env :=
-  fun var idx => match (string_dec var v, Nat.eqb idx i) with
-                 | (left _, true) => s
-                 | _ => e var idx
-                 end.
-Definition get_env (e: env) (v: var) (i: nat) : sexp_value := e v i.
+Check Compare_dec.lt_eq_lt_dec.
 
-Inductive Env : Set :=
-| BaseEnv : Env
-| RecEnv : Env -> world -> env -> Env -> sexp_value -> Env.
-Definition empty_Env : Env := BaseEnv.
-Definition set_Env (E: Env) (w: world) (e: env) (child_E: Env) (p: sexp_value) : Env :=
-  RecEnv E w e child_E p.
+Fixpoint string_lt (l r: string) : Prop :=
+  match l, r with
+  | EmptyString, EmptyString => Logic.False
+  | EmptyString, _ => Logic.True
+  | String lh lr, String rh rr =>
+    match Compare_dec.lt_eq_lt_dec (Ascii.nat_of_ascii lh) (Ascii.nat_of_ascii rh) with
+    | inleft (left _) => Logic.True
+    | inleft (right _) => string_lt lr rr
+    | inright _ => Logic.False
+    end
+  | _, _ => Logic.False
+  end.
 
-Record EnvRes : Set :=
-  mkEnvRes {
-      getSigma    : env;
-      getEnvSigma : Env;
-      getEnvPrint : sexp_value
-    }.
+Module String_as_OT <: UsualOrderedType.
 
-Fixpoint get_Env (E: Env) (w: world) : EnvRes :=
-  match E with
-  | BaseEnv => mkEnvRes empty_env  empty_Env (exist _ EmptySet EmptySetIsValue)
-  | RecEnv rest m_world m_e m_E p =>
-    match string_dec w m_world with
-    | left _ => mkEnvRes m_e m_E p
-    | right _ => get_Env rest w
+  Definition t := string.
+
+  Definition eq := @eq string.
+  Definition eq_refl := @eq_refl t.
+  Definition eq_sym := @eq_sym t.
+  Definition eq_trans := @eq_trans t.
+
+  Definition lt := string_lt.
+
+  Lemma lt_trans : forall x y z : t, string_lt x y -> string_lt y z -> string_lt x z.
+  Proof.
+    intros x.
+    induction x; intros ; destruct z; crush; destruct y; crush.
+    specialize IHx with y z.
+    do 3 (edestruct Compare_dec.lt_eq_lt_dec; crush).
+    destruct s, s0; crush.
+    destruct s, s0; crush.
+  Qed.
+
+  Lemma lt_not_eq : forall x y : t, string_lt x y -> ~ eq x y.
+  Proof.
+    intros x.
+    induction x ; destruct y ; crush.
+    edestruct Compare_dec.lt_eq_lt_dec; crush.
+    unfold eq in H0.
+    destruct s. crush.
+    specialize IHx with y.
+    crush.
+  Qed.
+
+  Definition compare x y : OrderedType.Compare string_lt eq x y.
+  Proof.
+    generalize y.
+    clear y.
+    induction x; intros.
+    * destruct y.
+      - assert (eq "" "").
+        crush.
+        constructor 2. auto.
+      - constructor 1. crush.
+    * destruct y.
+      - constructor 3. crush.
+      - remember (Ascii.nat_of_ascii a) as an.
+        remember (Ascii.nat_of_ascii a0) as a0n.
+        specialize Ascii.ascii_nat_embedding with a.
+        specialize Ascii.ascii_nat_embedding with a0.
+        intros.
+        specialize IHx with y.
+        destruct Compare_dec.lt_eq_lt_dec with an a0n ;
+          try (destruct s) ;
+          inversion IHx;
+          [> constructor 1 ..
+          | constructor 2
+          | constructor 3
+          | constructor 3
+          | constructor 3
+          | constructor 3 ] ;
+          crush ;
+          edestruct Compare_dec.lt_eq_lt_dec;
+          crush.
+  Qed.
+
+  Definition eq_dec := string_dec.
+
+End String_as_OT.
+
+Module NodeVar_OT := PairOrderedType String_as_OT String_as_OT.
+Module NodeVarMap := FMapList.Make(NodeVar_OT).
+
+Definition var_store := NodeVarMap.t sexp_value.
+Definition var_store_stack := list var_store.
+Definition world_store := world -> option (var_store_stack * var_store).
+Definition principals := set node.
+Definition location := node.
+Definition handlers := op -> option (node * var * sexp).
+Definition mergers := node -> var -> option sexp.
+
+Definition empty_env : var_store := NodeVarMap.empty sexp_value.
+
+Definition set_env (e: var_store) (n: node) (v: var) (val: sexp_value) : var_store :=
+  NodeVarMap.add (n, v) val e.
+
+Definition get_env (e: var_store) (n: node) (v: var) : option sexp_value :=
+  NodeVarMap.find (n, v) e.
+
+Fixpoint lookup (env: var_store_stack) (n: node) (v: var) :=
+  match env with
+  | nil => None
+  | cons e rest =>
+    match get_env e n v with
+    | Some res => Some res
+    | None => lookup rest n v
     end
   end.
 
-Inductive sexp_step : sexp -> env -> nat -> sexp -> Prop :=
-| VarZeroStep : forall (sigma: env) (v: var),
-    sexp_step (Var v) sigma 0 (proj1_sig (sigma v 0))
-| VarGtStep : forall (sigma: env) (i: nat) (v: var) (s1 s2: sexp),
-    i > 0 -> (proj1_sig (sigma v i)) = s1 -> sexp_step (Var v) sigma (i - 1) s2 ->
-    sexp_step (Var v) sigma i (Extend s1 s2)
-| NullExtendStep : forall (sigma: env) (i: nat) (svp: sexp_value),
-    let sv := proj1_sig svp in
-    sexp_step (Extend EmptySet sv) sigma i sv
-| ExtendStep : forall (sigma: env) (i: nat) (svp1 svp2 svp3: sexp_value),
-    let sv1 := proj1_sig svp1 in
-    let sv2 := proj1_sig svp2 in
-    let sv3 := proj1_sig svp3 in
-    sexp_step (Extend (Cons sv1 sv2) sv3) sigma i (Cons sv1 (Extend sv2 sv3))
-| ContextSexp : forall (sigma: env) (i: nat) (ctx: sexp_evaluation_context) (s s': sexp),
-    sexp_step s sigma i s' ->
-    sexp_step (sexp_of_context ctx s) sigma i (sexp_of_context ctx s').
+Definition empty_world_store : world_store :=
+  fun _ => None.
 
-Inductive bool_step : bool -> env -> nat -> bool -> Prop :=
-| MemEmpty : forall (sigma: env) (i: nat) (svp: sexp_value),
-    let sv := proj1_sig svp in
-    bool_step (Mem sv EmptySet) sigma i False
-| MemCons : forall (sigma: env) (i: nat) (svp1 svp2 svp3: sexp_value),
-    let sv1 := proj1_sig svp1 in
-    let sv2 := proj1_sig svp2 in
-    let sv3 := proj1_sig svp3 in
-    bool_step (Mem sv1 (Cons sv2 sv3)) sigma i (Disj (Eq sv1 sv2) (Mem sv1 sv3))
-| EqEmpty : forall (sigma: env) (i: nat),
-    bool_step (Eq EmptySet EmptySet) sigma i True
-| EqCons : forall (sigma: env) (i: nat) (svp1 svp2 svp1' svp2': sexp_value),
-    let sv1 := proj1_sig svp1 in
-    let sv2 := proj1_sig svp2 in
-    let sv1' := proj1_sig svp1' in
-    let sv2' := proj1_sig svp2' in
-    bool_step (Eq (Cons sv1 sv2) (Cons sv1' sv2')) sigma i (Conj (Eq sv1 sv1') (Eq sv2 sv2'))
-| EqNotL : forall (sigma: env) (i: nat) (svp1 svp2: sexp_value),
-    let sv1 := proj1_sig svp1 in
-    let sv2 := proj1_sig svp2 in
-    bool_step (Eq (Cons sv1 sv2) EmptySet) sigma i False
-| EqNotR : forall (sigma: env) (i: nat) (svp1 svp2: sexp_value),
-    let sv1 := proj1_sig svp1 in
-    let sv2 := proj1_sig svp2 in
-    bool_step (Eq EmptySet (Cons sv1 sv2)) sigma i False
-| ConjTrue: forall (sigma: env) (i: nat) (bvp: bool_value),
-    let bv := proj1_sig bvp in
-    bool_step (Conj True bv) sigma i bv
-| ConjFalse: forall (sigma: env) (i: nat) (bvp: bool_value),
-    let bv := proj1_sig bvp in
-    bool_step (Conj False bv) sigma i False
-| DisjTrue: forall (sigma: env) (i: nat) (bvp: bool_value),
-    let bv := proj1_sig bvp in
-    bool_step (Disj True bv) sigma i True
-| DisjFalse: forall (sigma: env) (i: nat) (bvp: bool_value),
-    let bv := proj1_sig bvp in
-    bool_step (Disj False bv) sigma i bv
-| ContextBoolSexp : forall (sigma: env) (i: nat) (ctx: bool_sexp_evaluation_context) (s s': sexp),
-    sexp_step s sigma i s' ->
-    bool_step (bool_of_bool_sexp_context ctx s) sigma i (bool_of_bool_sexp_context ctx s')
-| ContextBoolBool : forall (sigma: env) (i: nat) (ctx: bool_evaluation_context) (b b': bool),
-    bool_step b sigma i b' ->
-    bool_step (bool_of_bool_context ctx b) sigma i (bool_of_bool_context ctx b').
+Definition set_world_store (w: world_store) (u: world) (S: var_store_stack) (s: var_store) : world_store :=
+  fun u' =>
+    match string_dec u u' with
+    | left _ => Some (S, s)
+    | right _ => w u'
+    end.
 
-Inductive com_step : com -> env -> nat -> Env -> com -> env -> Env -> option sexp_value -> Prop :=
-| SeqStep : forall (sigma: env) (i: nat) (Sigma: Env) (c: com),
-    com_step (Seq Skip c) sigma i Sigma c sigma Sigma None
-| SeqProp : forall (sigma sigma': env) (i: nat) (Sigma Sigma': Env) (c1 c1' c2: com) (p: option sexp_value),
-    com_step c1 sigma i Sigma c1' sigma' Sigma' p ->
-    com_step (Seq c1 c2) sigma i Sigma (Seq c1' c2) sigma' Sigma' p
-| PrintStep : forall (sigma: env) (i: nat) (Sigma: Env) (svp: sexp_value),
-    let sv := proj1_sig svp in
-    com_step (Print sv) sigma i Sigma Skip sigma Sigma (Some svp)
-| PrintProp : forall (sigma: env) (i: nat) (Sigma: Env) (s s': sexp),
-    sexp_step s sigma i s' ->
-    com_step (Print s) sigma i Sigma (Print s') sigma Sigma None
-| IfTrue : forall (sigma: env) (i: nat) (Sigma: Env) (c1 c2: com),
-    com_step (If True c1 c2) sigma i Sigma c1 sigma Sigma None
-| IfFalse : forall (sigma: env) (i: nat) (Sigma: Env) (c1 c2: com),
-    com_step (If False c1 c2) sigma i Sigma c2 sigma Sigma None
-| IfProp : forall (sigma: env) (i: nat) (Sigma: Env) (c1 c2: com) (b b': bool),
-    bool_step b sigma i b' ->
-    com_step (If b c1 c2) sigma i Sigma (If b' c1 c2) sigma Sigma None
-| Assgn : forall (sigma: env) (i: nat) (Sigma: Env) (v: var) (svp: sexp_value),
-    let sv := proj1_sig svp in
-    let svph := proj2_sig svp in
-    let prev := sigma v i in
-    let prevv := proj1_sig prev in
-    let prevp := proj2_sig prev in
+Definition empty_handlers : handlers :=
+  fun _ => None.
 
-    let new : sexp_value := exist _ (Cons sv prevv) (ConsValuesIsValue _ _ svph prevp) in
+Definition set_handler (h: handlers) (o: op) (n: node) (v: var) (s: sexp) : handlers :=
+  fun o' =>
+    match string_dec o o' with
+    | left _ => Some (n, v, s)
+    | right _ => h o'
+    end.
 
-    com_step (Assign v sv) sigma i Sigma Skip (set_env sigma v i new) Sigma None
-| AssgnProp : forall (sigma: env) (i: nat) (Sigma: Env) (v: var) (s s': sexp),
-    sexp_step s sigma i s' ->
-    com_step (Assign v s) sigma i Sigma (Assign v s') sigma Sigma None
-| HypSkip : forall (sigma: env) (i: nat) (Sigma: Env) (w: world),
-    com_step (Hyp w Skip) sigma i Sigma Skip sigma Sigma None
-| HypProp : forall (sigma sigma_h': env) (i: nat) (Sigma Sigma_h': Env) (w: world) (c c': com) (p: option sexp_value),
-    let res := get_Env Sigma w in
-    let sigma_h := getSigma res in
-    let Sigma_h := getEnvSigma res in
-    let p_h := getEnvPrint res in
+Definition empty_mergers : mergers :=
+  fun _ _ => None.
 
-    let p_hs := proj1_sig p_h in
-    let p_hp := proj2_sig p_h in
+Definition set_merger (m: mergers) (n: node) (v: var) (s: sexp) : mergers :=
+  fun n' v' =>
+    match (string_dec n n', string_dec v v') with
+    | (left _, left _) => Some s
+    | _ => m n' v'
+    end.
 
-    com_step c sigma_h (i + 1) Sigma_h c' sigma_h' Sigma_h' p ->
-    let p_h' :=
-        match p with
-        | None => exist _ p_hs p_hp
-        | Some (exist _ ps pp) =>
-          exist _ (Cons ps p_hs) (ConsValuesIsValue _ _ pp p_hp)
+Program Fixpoint sexp_step (s: sexp) (env: var_store_stack) (pi: principals) : option sexp_value :=
+  match s with
+  | EmptySet => Some EmptySet
+  | Cons l r =>
+    match sexp_step l env pi, sexp_step r env pi with
+    | Some lv, Some rv =>
+      Some (Cons lv rv)
+    | _, _ => None
+    end
+  | Var n v =>
+    match set_mem string_dec n pi with
+    | true => lookup env n v
+    | false => None
+    end
+  end.
+Next Obligation.
+eapply ConsValuesIsValue; destruct (_: sexp_value); auto.
+Defined.
+
+Inductive bool_wf_rel : bool -> bool -> Prop :=
+| ConjWfL : forall (a b: bool), bool_wf_rel a (Conj a b)
+| ConjWfR : forall (a b: bool), bool_wf_rel b (Conj a b)
+| DisjWfL : forall (a b: bool), bool_wf_rel a (Disj a b)
+| DisjWfR : forall (a b: bool), bool_wf_rel b (Disj a b)
+| TrueWf : forall a, a <> True -> bool_wf_rel True a
+| FalseWf : forall a, a <> False -> bool_wf_rel False a
+| EqLtMem : forall elem elemv list env pi vl vr p1 p2,
+    sexp_step list env pi = Some (exist sexp_is_value (Cons vl vr) p1) ->
+    sexp_step elem env pi = Some (exist sexp_is_value elemv p2) ->
+    bool_wf_rel (Eq elemv vl) (Mem elem list)
+| MemLtMem : forall elem elemv list env pi vl vr p1 p2,
+    sexp_step list env pi = Some (exist sexp_is_value (Cons vl vr) p1) ->
+    sexp_step elem env pi = Some (exist sexp_is_value elemv p2) ->
+    bool_wf_rel (Mem elemv vr) (Mem elem list)
+| EqLtEqL : forall l r ll lr rl rr env pi p1 p2,
+    sexp_step l env pi = Some (exist sexp_is_value (Cons ll lr) p1) ->
+    sexp_step r env pi = Some (exist sexp_is_value (Cons rl rr) p2) ->
+    bool_wf_rel (Eq ll rl) (Eq l r)
+| EqLtEqR : forall l r ll lr rl rr env pi p1 p2,
+    sexp_step l env pi = Some (exist sexp_is_value (Cons ll lr) p1) ->
+    sexp_step r env pi = Some (exist sexp_is_value (Cons rl rr) p2) ->
+    bool_wf_rel (Eq lr rr) (Eq l r).
+Hint Constructors bool_wf_rel.
+
+Fixpoint measure_sexp_value (s: sexp) :=
+  match s with
+  | EmptySet => 1
+  | Var _ _ => 1
+  | Cons l r =>
+    measure_sexp_value l +
+    measure_sexp_value r
+  end.
+
+Theorem measure_sexp_value_positive : forall s, measure_sexp_value s > 0.
+Proof.
+  induction s; crush.
+Qed.
+
+Fixpoint measure_bool_psuedovalue (b: bool) :=
+  match b with
+  | True => 0
+  | False => 0
+  | Conj l r => 1 + measure_bool_psuedovalue l + measure_bool_psuedovalue r
+  | Disj l r => 1 + measure_bool_psuedovalue l + measure_bool_psuedovalue r
+  | Mem l r => 1 + measure_sexp_value l + measure_sexp_value r
+  | Eq l r => 1 + measure_sexp_value l + measure_sexp_value r
+  end.
+
+Program Fixpoint bool_psuedovalue_step (b: bool_psuedovalue) (env: var_store_stack) (pi: principals) {measure (measure_bool_psuedovalue b)} : option bool_value :=
+  match b with
+  | True => Some True
+  | False => Some False
+  | Eq EmptySet EmptySet => Some True
+  | Eq (Cons ll lr) (Cons rl rr) =>
+    match bool_psuedovalue_step (Eq ll rl) env pi as leq,
+          bool_psuedovalue_step (Eq lr rr) env pi as req with
+    | (Some (exist _ True _)), (Some (exist _ True _)) => Some True
+    | Some _, Some _ => Some False
+    | _, _ => None
+    end
+  | Eq (Var _ _) _ => None
+  | Eq _ (Var _ _) => None
+  | Eq _ _ => Some False
+  | Mem (Var _ _) _ => None
+  | Mem _ (Var _ _) => None
+  | Mem _ EmptySet => Some False
+  | Mem l (Cons rl rr) =>
+    match bool_psuedovalue_step (Eq l rl) env pi as leq,
+          bool_psuedovalue_step (Mem l rr) env pi as rmem with
+    | (Some (exist _ False _)), (Some (exist _ False _)) => Some False
+    | Some _, Some _ => Some True
+    | _, _ => None
+    end
+  | Conj l r =>
+    match bool_psuedovalue_step l env pi as lv,
+          bool_psuedovalue_step l env pi as rv with
+    | (Some (exist _ True _)), (Some (exist _ True _)) => Some True
+    | Some _, Some _ => Some False
+    | _, _ => None
+    end
+  | Disj l r =>
+    match bool_psuedovalue_step l env pi as lv,
+          bool_psuedovalue_step l env pi as rv with
+    | Some (exist _ False _), Some (exist _ False _) => Some False
+    | Some _, Some _ => Some True
+    | _, _ => None
+    end
+  end.
+Ltac pseudovalue_prover b :=
+  (
+    destruct b;
+    inversion b; crush;
+    constructor;
+    inversion H; eauto;
+    inversion H0; eauto
+  ).
+
+Solve All Obligations with (pseudovalue_prover b).
+
+Ltac arith_prover :=
+  crush;
+  match goal with
+  | [H1: sexp, H2: sexp, H3: sexp |- _] =>
+    specialize measure_sexp_value_positive with H1;
+    specialize measure_sexp_value_positive with H2;
+    specialize measure_sexp_value_positive with H3;
+    crush
+  end.
+Obligation Tactic := Tactics.program_simpl; intros; arith_prover.
+Solve Obligations.
+Obligation Tactic := Tactics.program_simpl.
+
+Program Fixpoint bool_to_psuedovalue (b: bool) (env: var_store_stack) (pi: principals) : option bool_psuedovalue :=
+  match b with
+  | True => Some True
+  | False => Some False
+  | Conj l r =>
+    match bool_to_psuedovalue l env pi, bool_to_psuedovalue r env pi with
+    | Some lv, Some rv => Some (Conj lv rv)
+    | _, _ => None
+    end
+  | Disj l r =>
+    match bool_to_psuedovalue l env pi, bool_to_psuedovalue r env pi with
+    | Some lv, Some rv => Some (Disj lv rv)
+    | _, _ => None
+    end
+  | Eq l r =>
+    match sexp_step l env pi, sexp_step r env pi with
+    | Some lv, Some rv => Some (Eq lv rv)
+    | _, _ => None
+    end
+  | Mem l r =>
+    match sexp_step l env pi, sexp_step r env pi with
+    | Some lv, Some rv => Some (Mem lv rv)
+    | _, _ => None
+    end
+  end.
+Next Obligation.
+  destruct b1.
+  destruct b0.
+  crush.
+Defined.
+Next Obligation.
+  destruct b1.
+  destruct b0.
+  crush.
+Defined.
+Next Obligation.
+  destruct lv.
+  destruct rv.
+  crush.
+Defined.
+Next Obligation.
+  destruct lv.
+  destruct rv.
+  crush.
+Defined.
+
+Inductive result : Type -> Type :=
+  fun typ => {typ} + {string}.
+
+Definition bool_step (b: bool) (env: var_store_stack) (pi: principals) : option bool_value :=
+  match bool_to_psuedovalue b env pi with
+  | Some bv => bool_psuedovalue_step bv env pi
+  | None => None
+  end.
+
+Open Scope string_scope.
+
+Definition merge_variable (Sig_o Sig_t: var_store_stack) (pi: principals) (mu: mergers) (key: node*var) (hval: sexp_value) (optsig: option var_store) : option var_store :=
+  let (n, v) := key in
+  let orig_var := lookup Sig_o n v in
+  let curr_var := lookup Sig_t n v in
+  let sho := mu n v in
+  match optsig, orig_var, curr_var, sho with
+  | Some acc, Some oval, Some cval, Some sh =>
+    let hsig := set_env empty_env "scratch" "hypo" hval in
+    let osig := set_env hsig "scratch" "orig" oval in
+    let csig := set_env osig "scratch" "curr" cval in
+    match sexp_step sh (cons csig Sig_t) pi with
+    | Some val =>
+      Some (set_env acc n v val)
+    | None => None
+    end
+  | Some acc, _, _, _ => Some acc
+  | _, _, _, _ => None
+  end.
+
+Fixpoint com_step (c: com) (sigma: var_store) (Sigma: var_store_stack) (omega: world_store) (pi: principals) (rho: location) (eta: handlers) (mu: mergers) : option (var_store * world_store) :=
+  match c with
+  | Skip => Some (sigma, omega)
+  | Seq l r =>
+    match com_step l sigma Sigma omega pi rho eta mu with
+    | Some (sigma', omega') =>
+      com_step r sigma' Sigma omega' pi rho eta mu
+    | None => None
+    end
+  | If b t f =>
+    match bool_step b (cons sigma Sigma) pi as b' with
+    | Some (exist _ True _) => com_step t sigma Sigma omega pi rho eta mu
+    | Some (exist _ False _) => com_step f sigma Sigma omega pi rho eta mu
+    | _ => None
+    end
+  | With n c' =>
+    com_step c' sigma Sigma omega (cons n pi) rho eta mu
+  | At n c' =>
+    com_step c' sigma Sigma omega pi n eta mu
+  | Handle n v op sh sm c' =>
+    let eta' := set_handler eta op n v sh in
+    let mu' := set_merger mu n v sm in
+    com_step c' sigma Sigma omega pi rho eta' mu'
+  | Op op =>
+    match eta op with
+    | Some (n, v, s) =>
+      match sexp_step s (cons sigma Sigma) pi with
+      | Some s' =>
+        match set_mem string_dec n pi with
+        | true =>
+          let sigma' := set_env sigma n v s' in
+          Some (sigma', omega)
+        | false =>
+          None
         end
-    in
-    let Sigma' := set_Env Sigma w sigma_h' Sigma_h' p_h' in
+      | None => None
+      end
+    | None => None
+    end
+  | Hyp w c =>
+    match com_step c empty_env (cons sigma Sigma) empty_world_store pi rho eta mu with
+    | Some (sigma', omega') =>
+      let omega'' := set_world_store omega w (cons sigma Sigma) sigma' in
+      Some (sigma, omega')
+    | None => None
+    end
+  | Commit w =>
+    match omega w with
+    | Some (Sigma_o, sigma_h) =>
+      let merge_fold := (merge_variable Sigma_o (cons sigma Sigma) (cons "scratch" pi) mu) in
+      match NodeVarMap.fold merge_fold sigma_h (Some sigma) with
+      | Some sigma' => Some (sigma', omega)
+      | None => None
+      end
+    | None => None
+    end
+  end.
 
-    com_step (Hyp w c) sigma i Sigma (Hyp w c') sigma Sigma' None
-| CommitVars : forall (sigma: env) (i: nat) (Sigma: Env) (w: world) (s1 s2: sexp_value) (v: var),
-    let sv1 := proj1_sig s1 in
-    let sp1 := proj2_sig s1 in
-    let sv2 := proj1_sig s2 in
-    let sp2 := proj2_sig s2 in
 
-    let cons_value := exist _ (Cons sv1 sv2) (ConsValuesIsValue _ _ sp1 sp2) in
+Definition run (c: com) :=
+  match com_step c empty_env nil empty_world_store nil "" empty_handlers empty_mergers with
+  | Some (sigma, omega) => Some sigma
+  | None => None
+  end.
 
-    sigma v (i + 1) = cons_value ->
-    let res := get_Env Sigma w in
-    let sigma_h := getSigma res in
-    let Sigma_h := getEnvSigma res in
-    let p_h := getEnvPrint res in
+Definition test_com := (With "Alice" (Seq (Handle "alice" "times" "%tmp" (Cons EmptySet (Cons EmptySet (Cons EmptySet (Cons EmptySet EmptySet)))) EmptySet (Op "%tmp")) (With "Bob" (Seq (Handle "bob" "times" "%tmp" (Cons EmptySet (Cons EmptySet (Cons EmptySet (Cons EmptySet EmptySet)))) EmptySet (Op "%tmp")) (With "Alice" (Seq (Handle "alice" "fitness" "%tmp" EmptySet EmptySet (Op "%tmp")) (Handle "alice" "fitness" "set_fitness" (Cons (Var "alice" "fitness") (Var "bob" "fitness")) (Cons (Var "scratch" "orig") (Cons (Var "scratch" "hypo") (Var "scratch" "curr"))) (Hyp "world" (Seq (At "DataCenter" (With "Bob" (Op "set_fitness"))) (Commit "world")))))))))).
 
-    let sigma_h' := set_env sigma_h v (i + 1) s2 in
-    let Sigma' := set_Env Sigma w sigma_h' Sigma_h p_h in
-    com_step (Commit w) sigma i Sigma (Seq (Assign v sv1) (Commit w)) sigma Sigma' None
-| CommitPrints : forall (sigma: env) (i: nat) (Sigma: Env) (w: world) (s1 s2: sexp_value),
-    let sv1 := proj1_sig s1 in
-    let sp1 := proj2_sig s1 in
-    let sv2 := proj1_sig s2 in
-    let sp2 := proj2_sig s2 in
-
-    let res := get_Env Sigma w in
-    let sigma_h := getSigma res in
-    let Sigma_h := getEnvSigma res in
-    let p_h := getEnvPrint res in
-
-    p_h = (exist _ (Cons sv1 sv2) (ConsValuesIsValue _ _ sp1 sp2)) ->
-
-    let Sigma' := set_Env Sigma w sigma_h Sigma_h s2 in
-
-    forall (v: var), (proj1_sig (sigma_h v (i + 1))) = EmptySet ->
-                     com_step (Commit w) sigma i Sigma
-                              (Seq (Print sv1) (Commit w)) sigma Sigma' None
-
-| CommitDone : forall (sigma: env) (i: nat) (Sigma: Env) (w: world),
-    let res := get_Env Sigma w in
-    let sigma_h := getSigma res in
-    let Sigma_h := getEnvSigma res in
-    let p_h := getEnvPrint res in
-
-    p_h = (exist _ EmptySet EmptySetIsValue) ->
-    forall (v: var), (proj1_sig (sigma_h v (i + 1))) = EmptySet ->
-                     com_step (Commit w) sigma i Sigma
-                              (Skip) sigma Sigma None.
+Eval compute in (run test_com).
